compatibility warning removed, renamed Streams to Stream and the channel-datatype-stuff has its own theory/Root-file

src/inc/Channel.thy
@@ -1,81 +1,29 @@
 theory Channel
 
-imports HOLCF
+imports HOLCF user.Datatypes
 begin
-default_sort type
 
-section \<open>channel definition\<close>
-
-datatype channel = c1 | c2 | c3 | c4 | c5 | c6 | c7 | c8 | c9 | c10 | cbotNOPE | SomeBig nat
-
-datatype M = nat | eps | B bool
-instance M :: countable
-  apply(intro_classes)
-  by(countable_datatype)
-
-
-text \<open>wird generiert\<close>
-definition ctype :: "channel \<Rightarrow> M set" where 
-"ctype  = undefined"
 
 definition cEmpty :: "channel set" where
 "cEmpty = {c. ctype c = {}}"
 
-(* Axiom :D wird vom generator erfüllt*)
-lemma ctype_ax1:"\<exists>c. ctype c = {}"
-  oops (* Braucht man nur für "minus" Datentyp *)
-
 
 class chan =
-(* fixes Abs :: "channel \<Rightarrow> 'a" *)
-fixes Rep :: "'a \<Rightarrow> channel"
-(* assumes chan_type:"type_definition Rep Abs (range Rep)"  *)
-assumes chan_botsingle:"\<And>c. (range Rep)\<subseteq> cEmpty \<or> (range Rep)\<inter>cEmpty = {}" (* TODO: geht das schöner ? *)
-assumes chan_inj:"inj Rep"
+  fixes Rep :: "'a \<Rightarrow> channel"
+
+
+  assumes chan_botsingle:
+      "\<And>c.   (range Rep) \<subseteq> cEmpty 
+           \<or> (range Rep) \<inter> cEmpty = {}" 
+
+  assumes chan_inj:"inj Rep"
+
 begin
 
-abbreviation "Abs \<equiv> inv Rep"
+  abbreviation "Abs \<equiv> inv Rep"
 end
 
 
-(*
-(*example 1*)
-typedef myPortIn = "{cbotNOPE}"
-  apply auto
-  done
-
-instantiation myPortIn::chan
-begin
-definition "Abs = Abs_myPortIn"
-definition "Rep = Rep_myPortIn"
-instance
-  apply(standard)
-  oops
-  using Abs_myPortIn_def Rep_myPortIn_def type_definition.Rep_range type_definition_myPortIn apply fastforce
-  using Rep_myPortIn_def type_definition.Rep_range type_definition_myPortIn apply fastforce
-  by simp
-end
-
-
-(*example 2*)
-typedef myPortOut = "{c1,c2,c3}"
-  apply auto
-  done
-
-
-section \<open>chan instantiations \<close>
-
-instantiation myPortOut::chan
-begin
-definition "Abs = Abs_myPortOut"
-definition "Rep = Rep_myPortOut"
-instance
-  apply(standard)
-  oops
-  using Abs_myPortOut_def Rep_myPortOut_def type_definition.Rep_range type_definition_myPortOut apply fastforce
-  using Rep_myPortOut_def type_definition.Rep_range type_definition_myPortOut apply fastforce
-  by simp
-end
 
 section \<open> rep abs chan lemmata \<close>
 
@@ -84,20 +32,11 @@ lemma repinrange[simp]:"Rep (c::'c::chan) = x \<Longrightarrow> x\<in> range(Rep
 
 lemma chan_eq[simp]:"Rep (c::'c::chan) = x \<Longrightarrow> x\<in> range(Rep::'d::chan \<Rightarrow> channel) 
                         \<Longrightarrow> Rep((Abs::channel \<Rightarrow> 'd)(Rep c)) = x"
-  by (meson chan_type type_definition_def)
+  by (simp add: f_inv_into_f)
+
+
 
 (*
-instantiation channel :: chan 
-begin 
-definition "Abs == id" 
-definition "Rep == (\<lambda> c. if c = cbot then c10 else c)"
-instance
-  apply intro_classes
-  using type_definition.Rep_range type_definition_channel Abs_channel_def Rep_channel_def
-  apply (smt channel.distinct(127) image_iff)
-  by simp
-end
-*)
 declare[[show_types]]
 declare[[show_consts]]
 
@@ -109,73 +48,33 @@ typedef ('c1::chan, 'c2::chan) union (infixr "\<union>" 20) = "if range (Rep::'c
   done
 
 (* Axiom :/ *)
-lemma "cEmpty \<noteq> {}"
+lemma cempty_exists: "cEmpty \<noteq> {}"
   sorry
 
 typedef ('c1::chan, 'c2::chan) minus (infixr "-" 20) = "(if range (Rep::'c1\<Rightarrow>channel) \<subseteq> range (Rep::'c2\<Rightarrow>channel) then cEmpty
                                                          else range (Rep::'c1\<Rightarrow>channel) - range (Rep::'c2\<Rightarrow>channel))" 
-  sorry
-
-lemma "False"
-  oops
+apply(cases "range Rep \<subseteq> range Rep", auto)
+  using cempty_exists by blast+
 
 instantiation union :: (chan, chan) chan 
 begin
-definition "Abs == Abs_union"
 definition "Rep == Rep_union"
 instance
   apply intro_classes
-  apply (smt Abs_union_def Rep_union_def type_definition.Rep_range type_definition_union)
-  apply (smt Diff_iff Rep_union_def singletonD singletonI type_definition.Rep_range type_definition_union)
-  by simp
+  apply auto
+  apply (metis (full_types) Diff_iff Rep_union Rep_union_def)
+  by (simp add: Channel.Rep_union_def Rep_union_inject inj_on_def)
 end
-
-section \<open> union range lemmata \<close>
-
-lemma union_bot[simp]:"cbot \<in> range (Rep::'a::chan\<Rightarrow>channel) \<and> cbot \<in> range (Rep::'b::chan\<Rightarrow>channel) 
-                       \<Longrightarrow> range (Rep::'a\<union>'b \<Rightarrow> channel) = {cbot}"
-  by (smt Rep_union_def type_definition.Rep_range type_definition_union)
-
-lemma union_notbot[simp]:"\<not>(cbot \<in> range (Rep::'a::chan\<Rightarrow>channel) \<and> cbot \<in> range (Rep::'b::chan\<Rightarrow>channel)) 
-                          \<Longrightarrow> range (Rep::'a\<union>'b \<Rightarrow> channel) \<noteq> {cbot}"
-  by (smt DiffE Rep_union_def singletonI type_definition.Rep_range type_definition_union)
-
-lemma union_isunionwithoutbot[simp]:"\<not>(cbot \<in> range (Rep::'a::chan\<Rightarrow>channel) \<and> cbot \<in> range (Rep::'b::chan\<Rightarrow>channel)) 
-                            \<Longrightarrow> range (Rep::'a\<union>'b \<Rightarrow> channel) = (range (Rep::'a::chan\<Rightarrow>channel)) \<union> range (Rep::'b::chan\<Rightarrow>channel) - {cbot}"
-  by (smt DiffE Rep_union_def singletonI type_definition.Rep_range type_definition_union)
-
-
-lemma union_isunion[simp]:"\<not>(cbot \<in> range (Rep::'a::chan\<Rightarrow>channel) \<or> cbot \<in> range (Rep::'b::chan\<Rightarrow>channel)) 
-                            \<Longrightarrow> range (Rep::'a\<union>'b \<Rightarrow> channel) = (range (Rep::'a::chan\<Rightarrow>channel)) \<union> range (Rep::'b::chan\<Rightarrow>channel)"
-  by simp
-
 
 instantiation minus :: (chan, chan) chan 
 begin
-definition "Abs == Abs_minus"
 definition "Rep == Rep_minus"
 instance
   apply intro_classes
-  apply (smt Abs_minus_def Rep_minus_def type_definition.Rep_range type_definition_minus)
-  apply(case_tac "c \<in> range (Rep::'b \<Rightarrow> channel)")
-  apply (smt Diff_iff Rep_minus_def singletonD type_definition.Rep_range type_definition_minus)
-  apply (smt DiffD1 Rep_minus_def chan_botsingle singleton_iff type_definition.Rep_range type_definition_minus)
-  by simp
+   apply auto
+  apply (metis (mono_tags, lifting) Diff_eq_empty_iff Diff_iff IntI Rep_minus Rep_minus_def chan_botsingle)
+  by (smt Rep_minus_def Rep_minus_inject injI)
 end
-
-section \<open> minus range lemmata \<close>
-
-lemma minus_bot[simp]:"range (Rep::'a::chan\<Rightarrow>channel) \<subseteq> range (Rep::'b::chan\<Rightarrow>channel) 
-                       \<Longrightarrow> range (Rep::'a-'b \<Rightarrow> channel) = {cbot}"
-  by (smt Rep_minus_def type_definition.Rep_range type_definition_minus)
-
-lemma minus_ismminus[simp]:"\<not>(range (Rep::'a::chan\<Rightarrow>channel) \<subseteq> range (Rep::'b::chan\<Rightarrow>channel)) 
-                            \<Longrightarrow> range (Rep::'a-'b \<Rightarrow> channel) = (range (Rep::'a::chan\<Rightarrow>channel)) - range (Rep::'b::chan\<Rightarrow>channel)"
-  by (smt Rep_minus_def type_definition.Rep_range type_definition_minus)
-
-lemma minus_bot2[simp]:"range (Rep::'a::chan\<Rightarrow>channel) = {cbot}
-                          \<Longrightarrow> range (Rep::'a-'b::chan \<Rightarrow> channel) = {cbot}"
-  by (smt Diff_iff chan_notempty minus_bot minus_ismminus subsetI subset_singletonD)
-
 *)
+
 end
