src/inc/Prelude.thy
@@ -1,4 +1,4 @@
-section {* Prelude *}
+section \<open>Prelude\<close>
 
 theory Prelude
 imports HOLCF
@@ -9,39 +9,39 @@ default_sort type
 (* allows to use lift_definition for continuous functions *)
 setup_lifting type_definition_cfun
 
-text {* Helpful lemmas to work with HOL and HOLCF's definitions.*}
+text \<open>Helpful lemmas to work with HOL and HOLCF's definitions.\<close>
 
 lemma trivial[simp]: "(Not \<circ> Not) = id"
   by auto
 
-text {* Convert a relation to a map (function with @{text "option"}al result).*}
+text \<open>Convert a relation to a map (function with \<open>option\<close>al result).\<close>
 definition rel2map ::   "('c * 'm) set \<Rightarrow> ('c \<rightharpoonup> 'm)"
 where rel2map_def: "rel2map r \<equiv> \<lambda>x. (if x \<in> Domain r then Some (SOME a. (x,a) \<in> r) else None)"
 
-text {* Domain of rel2map.*}
+text \<open>Domain of rel2map.\<close>
 lemma [simp]: "Map.dom (rel2map r) = Domain r"
 by (simp add: rel2map_def Map.dom_def)
 
-text {* Unwrapping an @{text "'a option"} value. Result for @{text "None"} is undefined.*}
+text \<open>Unwrapping an \<open>'a option\<close> value. Result for \<open>None\<close> is undefined.\<close>
 definition unsome :: "'a option \<Rightarrow> 'a" where
 "unsome x = (case x of Some y \<Rightarrow> y | None \<Rightarrow> undefined)"
 
-text {* Unsome is the inverse of Some.*}
+text \<open>Unsome is the inverse of Some.\<close>
 lemma [simp]: "unsome (Some x) = x"
 by (simp add: unsome_def)
 
-text {* For natural numbers j and k with @{term "j \<le> k"}, @{term "k - j"} is natural as well *}
+text \<open>For natural numbers j and k with @{term "j \<le> k"}, @{term "k - j"} is natural as well\<close>
 lemma natl1: "(j::nat) \<le> k \<Longrightarrow> \<exists>i. j + i = k"
 apply (simp add: atomize_imp)
 apply (rule_tac x="j" in spec)
 apply (induct_tac k, auto)
 by (case_tac "x", auto)
 
-text {* Commutation on natural numbers *}
+text \<open>Commutation on natural numbers\<close>
 lemma natl2: "(i::nat) + k = k + i"
 by auto
 
-text {* Removing successive duplicates from a list:*}
+text \<open>Removing successive duplicates from a list:\<close>
 primrec lrcdups :: "'a list \<Rightarrow> 'a list"
 where
   "lrcdups [] = []" |
@@ -55,12 +55,12 @@ where
 
 
 (* ----------------------------------------------------------------------- *)
-section {* Some auxiliary HOLCF lemmas *}
+section \<open>Some auxiliary HOLCF lemmas\<close>
 (* ----------------------------------------------------------------------- *)
 
 subsection \<open>cfun\<close> 
   
-text {* Introduction of continuity of @{text "f"} using monotonicity and lub on chains:*}
+text \<open>Introduction of continuity of \<open>f\<close> using monotonicity and lub on chains:\<close>
 lemma contI2:
   "\<lbrakk>monofun (f::'a::cpo \<Rightarrow> 'b::cpo); 
         (\<forall>Y. chain Y \<longrightarrow> f (\<Squnion>i. Y i) \<sqsubseteq> (\<Squnion>i. f (Y i)))\<rbrakk> \<Longrightarrow> cont f"
@@ -74,8 +74,8 @@ apply (rule_tac y="\<Squnion>i. f (Y i)" in below_trans, assumption)
 apply (rule is_lub_thelub)
 by (rule ch2ch_monofun [of f], assumption+)
 
-text {* The higher-order function, which takes as input f and yields the result of 
-the application of on x, is a continous function. *}
+text \<open>The higher-order function, which takes as input f and yields the result of 
+the application of on x, is a continous function.\<close>
 lemma [simp]: "cont (\<lambda> f. f x)"
 apply (rule contI)
 apply (subst lub_fun, assumption)
@@ -83,7 +83,7 @@ apply (rule thelubE)
 apply (rule ch2ch_fun, assumption)
 by (rule refl)
 
-text {* In a chain, every two elements are comparable *}
+text \<open>In a chain, every two elements are comparable\<close>
 lemma chain_tord: "chain S \<Longrightarrow> S k \<sqsubseteq> S j \<or> S j \<sqsubseteq> S k"
 apply (insert linear [of "j" "k"])
 apply (erule disjE)
@@ -92,7 +92,7 @@ apply (rule chain_mono,simp+)
 apply (rule disjI1)
 by (rule chain_mono,simp+)
 
-text {* Every non-empty set contains an element *}
+text \<open>Every non-empty set contains an element\<close>
 lemma neq_emptyD: "s \<noteq> {} \<Longrightarrow> \<exists>x. x \<in> s"
 by auto
 
@@ -112,31 +112,31 @@ lemma cfun_arg_eqI:  assumes "(a = b)"
 
      
 (* ----------------------------------------------------------------------- *)
-section {* More functions *}
+section \<open>More functions\<close>
 (* ----------------------------------------------------------------------- *)
 
-text {* This section introduces some more functions to work with lists.*}
+text \<open>This section introduces some more functions to work with lists.\<close>
 
-text {* Range shifting on least upper bound of chains. *}
+text \<open>Range shifting on least upper bound of chains.\<close>
 lemma less_lubl1: 
   "\<lbrakk>chain (Y::nat \<Rightarrow> 'a::cpo); X \<sqsubseteq> (\<Squnion>k. Y (k + j))\<rbrakk> \<Longrightarrow> X \<sqsubseteq> (\<Squnion>k. Y k)"
 by (subst lub_range_shift [THEN sym, of "Y" "j"], simp+)
 
-text {* Another lemma on range shifting on least upper bound of chains. *}
+text \<open>Another lemma on range shifting on least upper bound of chains.\<close>
 lemma less_lubl2:
 "\<lbrakk>chain (Y::nat \<Rightarrow> 'a::cpo); chain f; \<And>x. (\<Squnion>k. f k\<cdot>x) = x; \<And>n. f n\<cdot>x \<sqsubseteq> (f n\<cdot>(Lub Y))\<rbrakk> \<Longrightarrow> x \<sqsubseteq> Lub Y"
 by (insert lub_mono [of "\<lambda>n. f n\<cdot>x" "\<lambda>n. f n\<cdot>(Lub Y)"], simp)
 
-text {* Using the constructur Suc, show that n + 1 = 1 + n. *}
+text \<open>Using the constructur Suc, show that n + 1 = 1 + n.\<close>
 lemma Suc2plus: "Suc n = Suc 0 + n"
 by simp
 
-text {* Similar lemma as above, using the constructur Suc. *}
+text \<open>Similar lemma as above, using the constructur Suc.\<close>
 lemma Suc_def2: "Suc i = i + Suc 0"
 by simp
 
-text {* If a chain contains its least upper bound as an element, this element is the
-  maximum of the chain *}
+text \<open>If a chain contains its least upper bound as an element, this element is the
+  maximum of the chain\<close>
 lemma max_in_chainI3: "\<lbrakk>chain (Y::nat\<Rightarrow>'a::cpo); Y i = Lub Y\<rbrakk> \<Longrightarrow> max_in_chain i Y"
 apply (simp add: max_in_chain_def)
 apply (rule allI, rule impI)
@@ -146,28 +146,28 @@ apply (drule sym, simp)
 apply (rule chain_mono, assumption+)
 by (rule is_ub_thelub)
 
-text {* A chain which contains its maximum is finite *}
+text \<open>A chain which contains its maximum is finite\<close>
 lemma finite_chainI: "\<lbrakk>chain Y; max_in_chain i Y\<rbrakk> \<Longrightarrow> finite_chain Y"
 by (auto simp add: finite_chain_def)
 
-text {* 'zipping' two chains together also zips their least upper bounds *}
+text \<open>'zipping' two chains together also zips their least upper bounds\<close>
 lemma lub_prod2: "\<lbrakk>chain (X::nat \<Rightarrow> 'a::cpo); chain (Y::nat \<Rightarrow> 'b::cpo)\<rbrakk> \<Longrightarrow>
                         (\<Squnion>k. (X k,Y k)) = (Lub X, Lub Y)"
 by (subst lub_prod, simp+)
 
-text {* The least upper bound of a chainelement in a chain
-is the least upper bound of the chainelement plus another element*}
+text \<open>The least upper bound of a chainelement in a chain
+is the least upper bound of the chainelement plus another element\<close>
 lemma lub_range_shift2: "chain Y \<Longrightarrow> (\<Squnion>i. Y i) = (\<Squnion>i. Y (i+j))"
   apply(simp add: lub_def)
   using is_lub_range_shift lub_def by fastforce
   
 
-text{* The least upper bound of any finite chain is a member of the chain *}
+text\<open>The least upper bound of any finite chain is a member of the chain\<close>
 lemma l42: "chain S \<Longrightarrow> finite_chain S \<Longrightarrow> \<exists>t. (\<Squnion> j. S j) = S t"
 using lub_eqI lub_finch2 by auto
 
-text{* The least upper bound of a monotone function applied on a finite chain is the
-function applied to the least upper bound of the finite chain *}
+text\<open>The least upper bound of a monotone function applied on a finite chain is the
+function applied to the least upper bound of the finite chain\<close>
 lemma finite_chain_lub: fixes Y :: "nat \<Rightarrow> 'a ::cpo"
   assumes "finite_chain Y" and "chain Y" and "monofun f"
   shows "f (\<Squnion>i. Y i) = (\<Squnion>i. f (Y i))"
@@ -203,24 +203,24 @@ proof -
     using k_def by blast 
 qed     
 
-text {* Creating a list from iteration a function @{text "f"} 
-  @{text "n"}-times on a start value @{text s}.*}
+text \<open>Creating a list from iteration a function \<open>f\<close> 
+  \<open>n\<close>-times on a start value \<open>s\<close>.\<close>
 primrec literate :: "nat \<Rightarrow> ('a \<Rightarrow> 'a) \<Rightarrow> 'a \<Rightarrow> 'a list"
 where
   literate_0:  "literate 0 f s = []" |
   literate_Suc:"literate (Suc n) f s = s#(literate n f (f s))"
 
-text {* Iterative conversion of @{term literate} result to a set *}
+text \<open>Iterative conversion of @{term literate} result to a set\<close>
 lemma literate_Suc2:
   "set (literate (Suc n) f s) = {s} \<union> set (literate n f (f s))"
 by auto
 
-text {* A set of successive natural numbers can be split into the smallest
-  number and the rest *}
+text \<open>A set of successive natural numbers can be split into the smallest
+  number and the rest\<close>
 lemma natl3: "{i. x \<le> i \<and> i < Suc n + x} = {x} \<union> {i. Suc x \<le> i \<and> i < Suc n + x}"
 by auto
 
-text {* Create set of natural numbers from k to n+k-1 by @{term literate} *}
+text \<open>Create set of natural numbers from k to n+k-1 by @{term literate}\<close>
 lemma literatel1 [simp]: 
   "set (literate n Suc k) = {i. k \<le> i \<and> i < (n + k)}"
 apply (rule_tac x="k" in spec)
@@ -230,22 +230,22 @@ apply (rule allI)
 apply (erule_tac x="Suc x" in allE)
 by (subst natl3, simp)
 
-text {* A list of length @{term n} contains at most @{term n} different elements *}
+text \<open>A list of length @{term n} contains at most @{term n} different elements\<close>
 lemma card_set_list_le_length: "card (set x) \<le> length x"
 apply (induct_tac x, simp+)
 by (simp add: card_insert_if)
 
-text {* @{term "literate n"} creates lists with length @{term n} *}
+text \<open>@{term "literate n"} creates lists with length @{term n}\<close>
 lemma [simp]: "length (literate n f k) = n"
 apply (rule_tac x="k" in spec)
 by (induct_tac n, simp+)
 
-text {* Zipping and unzipping on lists *}
+text \<open>Zipping and unzipping on lists\<close>
 lemma [simp]: "map snd (map (Pair k) a) = a"
 by (induct_tac a, simp+)
 
-text {* For a list @{term x}, each element in @{term "set x"} appears at some position in
-  @{term x} *}
+text \<open>For a list @{term x}, each element in @{term "set x"} appears at some position in
+  @{term x}\<close>
 lemma from_set_to_nth: "xa \<in> set x \<Longrightarrow> \<exists>k. x!k = xa \<and> k < length x"
 apply (simp add: atomize_imp)
 apply (induct_tac x, simp+) 
@@ -255,11 +255,11 @@ apply (rule impI, simp)
 apply (erule exE)
 by (rule_tac x="Suc k" in exI, simp)
 
-text {* Replacing a filter on lists by a stronger filter *}
+text \<open>Replacing a filter on lists by a stronger filter\<close>
 lemma filterl4: "\<lbrakk>\<And>x. Q x \<Longrightarrow> P x; filter P x = []\<rbrakk> \<Longrightarrow> filter Q x = []"
 by (simp add: atomize_imp, induct_tac x, auto)
 
-text {* Induction on lists from the right *}
+text \<open>Induction on lists from the right\<close>
 lemma list_rinduct_lemma: "\<forall>y. length y = k \<and> (P [] \<and> (\<forall>x xs. P xs \<longrightarrow> P (xs @ [x]))) \<longrightarrow> P y"
 apply (induct_tac k, simp)
 apply (rule allI)
@@ -272,31 +272,31 @@ by (case_tac "y = []", auto)
 
 
 (* ----------------------------------------------------------------------- *)
-section {* Some more lemmas about sets *}
+section \<open>Some more lemmas about sets\<close>
 (* ----------------------------------------------------------------------- *)
 
-text {* All subsets of a finite set are finite themselves *}
+text \<open>All subsets of a finite set are finite themselves\<close>
 lemma finite_subset1: "finite Y \<Longrightarrow> (\<forall>X. X \<subseteq> Y \<longrightarrow> finite X)"
   by (simp add: finite_subset)
 
-text {* Given an infinite and a finite set, the infinite one contains an element
-  which is not in the finite one *}
+text \<open>Given an infinite and a finite set, the infinite one contains an element
+  which is not in the finite one\<close>
 lemma ex_new_if_finitel1:
   "\<lbrakk>finite Y; \<not> finite X\<rbrakk> \<Longrightarrow> \<exists>a. a \<in> X \<and> a \<notin> Y"
 apply (rule ccontr, auto)
 apply (subgoal_tac "X \<subseteq> Y")
 by (frule_tac Y="Y" in finite_subset1, auto)
 
-text {* Create a finite set with @{text "n"} distinct continuously 
-  numbered entries from set @{text "A"}.*}
+text \<open>Create a finite set with \<open>n\<close> distinct continuously 
+  numbered entries from set \<open>A\<close>.\<close>
 primrec
   getinj:: "'a set \<Rightarrow> nat \<Rightarrow> (nat \<times> 'a) set"
 where
   "getinj A 0 = {(0,SOME x. x \<in> A)}" |
   "getinj A (Suc n) = {(Suc n, SOME x. x \<in> A \<and> x \<notin> (snd ` (getinj A n)))} \<union> getinj A n"
 
-text {* The result of @{term "getinj A n"} and its projections on the first or
-  second attribute are finite *}
+text \<open>The result of @{term "getinj A n"} and its projections on the first or
+  second attribute are finite\<close>
 
 lemma finite_getinjs[simp]: "finite (getinj A n)"
 by (induct_tac n, simp+)
@@ -307,16 +307,16 @@ by (induct_tac n, simp+)
 lemma finite_fst_getinjs[simp]: "finite (fst ` (getinj A n))"
 by (induct_tac n, simp+)
 
-text {* @{term "getinj A n"} only contains entries for numbers up to @{term n} *}
+text \<open>@{term "getinj A n"} only contains entries for numbers up to @{term n}\<close>
 lemma getinjs_l1: "\<forall>k. n < k \<longrightarrow> (k, x) \<notin> getinj A n"
 by (induct_tac n, simp+)
 
-text {* ...especially, it contains no entry for @{term "n+1"} *}
+text \<open>...especially, it contains no entry for @{term "n+1"}\<close>
 lemma [simp]: "(Suc n,x) \<notin> getinj A n"
 by (insert getinjs_l1 [of n x A], auto)
 
-text {* Projecting to the second component is an injective function on results
-  of @{term getinj} *}
+text \<open>Projecting to the second component is an injective function on results
+  of @{term getinj}\<close>
 lemma card_getinj_lemma[simp]: "\<not> finite A \<Longrightarrow> card (snd ` (getinj A n)) = card (getinj A n)"
 apply (induct_tac n, simp+)
 apply (rule someI2_ex)
@@ -326,11 +326,11 @@ by (rule finite_snd_getinjs, simp+)
 lemma inj_on_getinj: "\<not> finite A \<Longrightarrow> inj_on snd (getinj A n)"
 by (rule eq_card_imp_inj_on, simp+)
 
-text {* @{term "getinj X n"} maps @{term n} to something *}
+text \<open>@{term "getinj X n"} maps @{term n} to something\<close>
 lemma getinj_ex[simp]: "\<exists>a. (n,a) \<in> getinj X n"
 by (induct_tac n, simp+)
 
-text {* For a fixed set @{term "A"}, @{term "getinj A i"} is a chain *}
+text \<open>For a fixed set @{term "A"}, @{term "getinj A i"} is a chain\<close>
 lemma getinj_chain:
   "\<lbrakk>\<not> finite A; (j, x) \<in> getinj A j; j \<le> k\<rbrakk> \<Longrightarrow> (j, x) \<in> getinj A k"
 apply (simp add: atomize_imp)
@@ -338,11 +338,11 @@ apply (induct_tac k, auto)
 by (case_tac "j = Suc n", auto)
 
 (* ----------------------------------------------------------------------- *)
-section {* updis *}
+section \<open>updis\<close>
 (* ----------------------------------------------------------------------- *)
 
-text {* The @{term "updis"} command lifts an arbitrary type to a
-  discrete pointed partial order. *}
+text \<open>The @{term "updis"} command lifts an arbitrary type to a
+  discrete pointed partial order.\<close>
 abbreviation
   updis :: "'a \<Rightarrow> 'a discr u"
     where "updis \<equiv> (\<lambda>a. up\<cdot>(Discr a))" 
