src/bundle/sbElem.thy
@@ -1,6 +1,6 @@
 theory sbElem
 
-imports stream.Streams inc.Channel
+imports inc.Channel
 begin
 
 default_sort chan
@@ -12,7 +12,7 @@ fun sbElem_well :: "('c::chan \<Rightarrow> M) option \<Rightarrow> bool" where
 "sbElem_well None = ((Rep ` (UNIV::'c set)) \<subseteq> cEmpty)" |  (* Schöner? *)
 "sbElem_well (Some sbe) = (\<forall> c. sbe c \<in> ctype (Rep c))" (* cbot ist leer, daher wird das nie wahr sein für das leere Bündel *)
 
-text{*Type sbElem is can be interpreted as a Timeslice*}
+text\<open>Type sbElem is can be interpreted as a Timeslice\<close>
 typedef 'c::chan sbElem  ("(_\<^sup>\<surd>)" [1000] 999) = "{f:: ('c::chan \<Rightarrow> M) option. sbElem_well f}"
 proof(cases "((range (Rep::'c \<Rightarrow> channel) \<subseteq> cEmpty))")
   case True
@@ -30,7 +30,7 @@ next
     by blast
 qed
 
-text{*Instantiation of sbElem as a discrete cpo*}
+text\<open>Instantiation of sbElem as a discrete cpo\<close>
 instantiation  sbElem::(chan)discrete_cpo
 begin
 definition "below_sbElem = (\<lambda>(sbe1::'a sbElem) sbe2. (sbe1 = sbe2))"
@@ -42,19 +42,19 @@ setup_lifting type_definition_sbElem
 
 subsection \<open>sbElem functions\<close>
 
-text{*This function retrieves an element on channel e from the sbElem. This only works 
-      if Elements are allowed on channel e and channel e is also in type c*}
+text\<open>This function retrieves an element on channel e from the sbElem. This only works 
+      if Elements are allowed on channel e and channel e is also in type c\<close>
 definition sbegetch::"'e \<Rightarrow> 'c\<^sup>\<surd> \<Rightarrow> M"where (*works if sbe \<noteq> None* and 'e \<subseteq> 'c *)
 "sbegetch c = (\<lambda> sbe. ((the (Rep_sbElem sbe)) (Abs (Rep c))))"
 
 
-text{*This function Restricts the Domain of an sbElem. This works if the Domain to restrict to is 
-      smaller*}
+text\<open>This function Restricts the Domain of an sbElem. This works if the Domain to restrict to is 
+      smaller\<close>
 definition sbeRestrict::"'c\<^sup>\<surd> \<Rightarrow> 'd\<^sup>\<surd>"where 
 "sbeRestrict = (\<lambda>sbe. Abs_sbElem(Some (\<lambda>c. sbegetch c sbe)))"
 
 
-text{*This unites two sbElems. It works, if type e is a subset of the union of type c and d*}
+text\<open>This unites two sbElems. It works, if type e is a subset of the union of type c and d\<close>
 definition sbeUnion::"'c\<^sup>\<surd> \<Rightarrow> 'd\<^sup>\<surd> \<Rightarrow> 'e\<^sup>\<surd>"where 
 "sbeUnion = (\<lambda>sbe1 sbe2. Abs_sbElem (Some(\<lambda> c. if (Rep c \<in> (range (Rep ::'c \<Rightarrow> channel))) then 
                   sbegetch c sbe1 else  sbegetch c sbe2)))"
