src/user/Datatypes.thy
@@ -1,0 +1,42 @@
+theory Datatypes
+
+imports HOLCF
+
+begin
+
+default_sort type
+
+section \<open>Datatype\<close>
+text \<open>The channel-datatype is fixed before the proof begins.
+  This datatype contains every channel, that is used. There is no way to "dynamically" add
+ channels, except modifying this datatype\<close>
+
+datatype channel = DummyChannel nat
+
+hide_const DummyChannel
+
+
+section \<open>Message Definition\<close>
+
+text\<open>The same is true for the "Message" Datatype. Every kind of message has to be described here:\<close>
+datatype M = DummyMessage nat
+hide_const DummyMessage
+
+instance M :: countable
+  apply(intro_classes)
+  by(countable_datatype)
+
+
+
+
+text \<open>Then one describes the types of each channel. Only Messages included are allowed to be
+  transmitted\<close>
+definition ctype :: "channel \<Rightarrow> M set" where 
+"ctype = undefined"
+
+hide_fact ctype_def
+
+
+
+
+end
